small_step.v
@@ -93,18 +93,6 @@ Record state := {
   stack : LocalStack;
 }.
 
-Inductive state_contains_r : state → Resource → Prop :=
-  | state_mem_contains : ∀ mem s r, mem_contains_r mem r → state_contains_r {|
-      mem := mem; stack := s;
-  |} r
-  | state_stack_contains : ∀ mem s r, lstack_contains_r s r → state_contains_r {|
-      mem := mem; stack := s;
-  |} r
-.
-
-Definition tag_consistent (s : state) : Prop :=
-  ∀ (r : Resource) (p1 p2 : state_contains_r s r), p1 = p2.
-
 Inductive step : state → state → Prop :=
   | step_c : ∀ {s0 s1 : state} {i : Instr},
     step_local s0.(mem) s0.(stack) i s1.(mem) s1.(stack) →
